Theorems.v
@@ -21,64 +21,22 @@ Theorem absence_of_dangling_pointers :
 Admitted.
 
 
-Lemma iff_env_partial_order :
-    forall env env' v, env_partial_orderb env env' v = true <-> env_partial_order env env' v.
-Proof.
-    intros. destruct env eqn:Senv. destruct env' eqn:Senv'. split.
-    - intro H. unfold env_partial_orderb in H. simpl in H. destruct (ω v) eqn:Ev.
-        * destruct v0 eqn:Ev0 ; destruct (ω1 v) eqn:Ev' ; subst ; try discriminate ; destruct v1 eqn:Ev1 ; subst ;simpl in H ; try discriminate.
-            ** apply Int.mi_eq_iff in H.  apply sameInt with n ; simpl.
-                *** assumption.
-                *** rewrite H. assumption. 
-            ** simpl in H. subst ; try discriminate. apply Nat.eqb_eq in H. subst. 
-                apply sameMpz with n0 ; simpl ; assumption.
-            ** apply undefInt with n ; simpl.
-                *** assumption.
-                *** right. assumption.
-            ** apply undefInt with (Int.of_z 0 zeroinRange) ; simpl.
-                *** assumption.
-                *** left. assumption.
-            ** apply undefMpz with n ; simpl.
-                *** assumption.
-                *** right. assumption.
-            ** apply undefMpz with 0%nat ; simpl.
-                *** assumption.
-                *** left. assumption.
-        * apply none. assumption.
-    - intro H. inversion H ; unfold env_partial_orderb ; rewrite H0 ; simpl in *.
-     * rewrite H1. apply Int.mi_eq_iff. reflexivity.
-     * rewrite H1. apply Nat.eqb_refl.
-     * destruct H1 ; rewrite H1 ; reflexivity. 
-     * destruct H1 ; rewrite H1 ; reflexivity. 
-     * reflexivity.
-Qed.
-
-Corollary refl_env_partial_order : forall e, e ⊑ e.
-Proof.
-    intros . apply iff_env_partial_order. unfold env_partial_orderb. 
-    destruct e.
-    simpl. destruct (ω v). destruct v0 ; try reflexivity.
-    unfold same_values. apply Int.mi_eq_iff.
-    * reflexivity.
-    * unfold same_values. apply Nat.eqb_refl.
-    * reflexivity.
-Qed.
-
-Lemma eq_env_partial_order : 
-    forall e e' v z, e ⊑ e' ->  z <> UInt /\ z <> UMpz -> (fst e) v = Some z -> (fst e') v = Some z.
-Proof.
-    intros. destruct H with v ; rewrite H2 in H1 ; try injection H1 as Eq ; subst ; try assumption.
-    - destruct H0 as [uint _]. destruct uint. reflexivity.
-    - destruct H0 as [_ umpz]. destruct umpz. reflexivity.
-    - discriminate.
-Qed.   
-
 
 Lemma weakening_of_expression_semantics : 
 forall env e x,
     env ⊨ e => x <-> (forall env', env ⊑ env' ->  env' ⊨ e => x)
 .
 Proof.
+    assert (
+        eq_env_partial_order : forall e e' v z, e ⊑ e' ->  z <> UInt /\ z <> UMpz -> (fst e) v = Some z -> (fst e') v = Some z
+    ). 
+    {
+        intros. destruct H with v ; try assumption ; try rewrite H2 in H1 ; try injection H1 as Eq ; subst ; try assumption.
+        - destruct H0 as [uint _]. destruct uint. reflexivity.
+        - destruct H0 as [_ umpz]. destruct umpz. reflexivity.
+        - discriminate.
+    }
+
     split.
     - generalize dependent x. induction e.
         * intros v H env' Inc. inversion H. subst. apply E_Int.
@@ -100,5 +58,5 @@ Proof.
                 ++ apply IHe1 ; assumption.
                 ++ apply IHe2 ; assumption.
                 ++ assumption.
-    - intro. apply H. apply refl_env_partial_order.
+    - intro. apply H. constructor.
 Qed.
